src/Ext/ExprSubst.v
@@ -1,0 +1,465 @@
+(** This file contains generic functions for manipulating,
+ ** i.e. substituting and finding, unification variables
+ **)
+Require Import ExtLib.Core.RelDec.
+Require Import ExtLib.Data.List.
+Require Import ExtLib.Data.Bool.
+Require Import ExtLib.Data.HList.
+Require Import ExtLib.Data.ListNth.
+Require Import ExtLib.Tactics.Consider.
+Require Import ExtLib.Tactics.Injection.
+Require Import ExtLib.Tactics.EqDep.
+Require Import MirrorCore.EnvI.
+Require Import MirrorCore.Ext.Expr.
+Require Import MirrorCore.Ext.ExprLift.
+
+Set Implicit Arguments.
+Set Strict Implicit.
+
+(** Temporary **)
+Require Import FunctionalExtensionality.
+
+Section substU.
+  Variable u : uvar.
+  Variable e' : expr.
+
+  Fixpoint substU (under : nat) (e : expr) : expr :=
+    match e with
+      | Var _ => e
+      | Func _ _ => e
+      | Not e => Not (substU under e)
+      | Equal t l r => Equal t (substU under l) (substU under r)
+      | App l r => App (substU under l) (substU under r)
+      | Abs t e => Abs t (substU (S under) e)
+      | UVar u' =>
+        if u ?[ eq ] u' then
+          lift 0 under e'
+        else UVar u'
+    end.
+End substU.
+
+Section instantiate.
+  Variable T : Type.
+  Variable lookup : uvar -> T -> option expr.
+
+  Fixpoint instantiate (under : nat) (e : expr) (s : T) : expr :=
+    match e with
+      | Var _
+      | Func _ _ => e
+      | Not e => Not (instantiate under e s)
+      | Equal t l r => Equal t (instantiate under l s) (instantiate under r s)
+      | App l r => App (instantiate under l s) (instantiate under r s)
+      | Abs t e => Abs t (instantiate (S under) e s)
+      | UVar u =>
+        match lookup u s with
+          | None => UVar u
+          | Some e => lift 0 under e
+        end
+    end.
+
+  Theorem typeof_expr_instantiate : forall tfs tu tg s,
+    (forall u e',
+       lookup u s = Some e' ->
+       exists t',
+         nth_error tu u = Some t' /\
+         typeof_expr tfs tu tg e' = Some t') ->
+    forall e tg',
+      typeof_expr tfs tu (tg' ++ tg) (instantiate (length tg') e s) =
+      typeof_expr tfs tu (tg' ++ tg) e.
+  Proof.
+    induction e; simpl; intros;
+    repeat match goal with
+             | H : _ |- _ =>
+               rewrite H
+           end; auto.
+    { specialize (IHe (t :: tg')). simpl in *.
+      rewrite IHe. reflexivity. }
+    { consider (lookup u s); intros; simpl; auto.
+      specialize (H _ _ H0). destruct H.
+      intuition.
+      generalize (typeof_expr_lift tfs tu nil tg' tg e); simpl.
+      congruence. }
+  Qed.
+
+  Theorem exprD'_instantiate : forall ts (fs : functions ts) us gs' s,
+    (forall u e',
+       lookup u s = Some e' ->
+       exists tval,
+         nth_error us u = Some tval /\
+         ExprD.exprD fs us gs' e' (projT1 tval) = Some (projT2 tval)) ->
+    forall e t v,
+      let (tv',vs') := EnvI.split_env gs' in
+      match ExprD.exprD' fs us (v ++ tv') e t ,
+            ExprD.exprD' fs us (v ++ tv') (instantiate (length v) e s) t
+      with
+        | Some l , Some r => forall vs,
+                               l (hlist_app vs vs') = r (hlist_app vs vs')
+        | None , None => True
+        | _ , _ => False
+      end.
+  Proof.
+    unfold ExprD.exprD. intros ts fs us gs'.
+    destruct (split_env gs'). intros s Hlookup.
+    induction e; simpl; intros; autorewrite with exprD_rw; auto.
+    { 
+      
+      change (
+          let zzz z (pf : Some z = nth_error (v0 ++ x) v) cast :=
+              fun e : hlist (typD ts nil) (v0 ++ x) =>
+                           match
+                             pf in (_ = t'')
+                             return
+                             (match t'' with
+                                | Some t0 => typD ts nil t0
+                                | None => unit
+                              end -> typD ts nil t)
+                           with
+                             | eq_refl => fun x0 : typD ts nil z => cast x0
+                           end (hlist_nth e v)
+                in
+          match
+            match
+              nth_error (v0 ++ x) v as z
+              return
+              (z = nth_error (v0 ++ x) v ->
+               option (hlist (typD ts nil) (v0 ++ x) -> typD ts nil t))
+            with
+              | Some z =>
+                fun pf : Some z = nth_error (v0 ++ x) v =>
+                  match typ_cast_typ ts (fun x0 : Type => x0) nil z t with
+                    | Some cast =>
+                      Some (zzz z pf cast)
+                    | None => None
+                  end
+              | None => fun _ : None = nth_error (v0 ++ x) v => None
+            end eq_refl
+          with
+            | Some l =>
+              match
+                match
+                  nth_error (v0 ++ x) v as z
+                  return
+                  (z = nth_error (v0 ++ x) v ->
+                   option (hlist (typD ts nil) (v0 ++ x) -> typD ts nil t))
+                with
+                  | Some z =>
+                    fun pf : Some z = nth_error (v0 ++ x) v =>
+                      match typ_cast_typ ts (fun x0 : Type => x0) nil z t with
+                        | Some cast =>
+                          Some (zzz z pf cast)
+                        | None => None
+                      end
+                  | None => fun _ : None = nth_error (v0 ++ x) v => None
+                end eq_refl
+              with
+                | Some r =>
+                  forall vs : hlist (typD ts nil) v0,
+                    l (hlist_app vs h) = r (hlist_app vs h)
+                | None => False
+              end
+            | None =>
+              match
+                match
+                  nth_error (v0 ++ x) v as z
+                  return
+                  (z = nth_error (v0 ++ x) v ->
+                   option (hlist (typD ts nil) (v0 ++ x) -> typD ts nil t))
+                with
+                  | Some z =>
+                    fun pf : Some z = nth_error (v0 ++ x) v =>
+                      match typ_cast_typ ts (fun x0 : Type => x0) nil z t with
+                        | Some cast =>
+                          Some (zzz z pf cast)
+                        | None => None
+                      end
+                  | None => fun _ : None = nth_error (v0 ++ x) v => None
+                end eq_refl
+              with
+                | Some _ => False
+                | None => True
+              end
+          end).
+      intro zzz; clearbody zzz; revert zzz; gen_refl.
+      destruct (nth_error (v0 ++ x) v); auto.
+      destruct (typ_cast_typ ts (fun x0 : Type => x0) nil t0 t); auto. }
+    { destruct (nth_error fs f); auto.
+      destruct (type_apply ts (fenv f0) l nil (ftype f0) (fdenote f0)); auto.
+      destruct (typ_cast_typ ts (fun x0 : Type => x0) nil
+         (instantiate_typ l (ftype f0)) t); auto. }
+    { rewrite typeof_expr_instantiate.
+      { consider (typeof_expr (typeof_funcs fs) (typeof_env us) (v ++ x) e1); auto.
+        destruct t0; auto.
+        specialize (IHe1 (tvArr t0_1 t0_2) v).
+        specialize (IHe2 t0_1 v).
+        repeat match goal with
+                 | _ : context [ match ?X with _ => _ end ] |- _ =>
+                   consider X; try congruence; intros
+                 | |- context [ match ?X with _ => _ end ] =>
+                   consider X; try congruence; intros
+               end; auto.
+        inv_all; subst. rewrite IHe2. rewrite IHe1. reflexivity. }
+      { clear - Hlookup.
+        intros. specialize (Hlookup _ _ H).
+        destruct Hlookup. intuition.
+        rewrite nth_error_typeof_env.
+        rewrite H1.
+        eexists; split; eauto.
+        consider (ExprD.exprD' fs us x e' (projT1 x0)); try congruence; intros.
+        eapply ExprD.typeof_expr_exprD'. eauto. } }
+    { destruct t0; auto.
+      specialize (IHe t0_2 (t :: v)). simpl in *.
+      repeat match goal with
+                 | _ : context [ match ?X with _ => _ end ] |- _ =>
+                   consider X; try congruence; intros
+                 | |- context [ match ?X with _ => _ end ] =>
+                   consider X; try congruence; intros
+               end; inv_all; subst; auto.
+      eapply functional_extensionality. intros.
+      specialize (IHe (Hcons (p x0) vs)). simpl in *; auto. }
+    { specialize (Hlookup u).
+      destruct (lookup u s).
+      { unfold lookupAs.
+        destruct (Hlookup _ eq_refl); clear Hlookup.
+        intuition.
+        rewrite H0. destruct x0; simpl in *.
+        generalize (exprD'_lift fs us nil v x e t); simpl.
+        consider (x0 ?[ eq ] t); intros; subst.
+        { consider (ExprD.exprD' fs us x e t); try congruence; intros.
+          consider (ExprD.exprD' fs us (v ++ x) (lift 0 (length v) e) t);
+            consider (ExprD.exprD' fs us x e t); intuition; try congruence.
+          inv_all. rewrite typ_cast_typ_refl.
+          intros.
+          specialize (H5 Hnil vs h). simpl in *. subst; auto. }
+        { match goal with
+            | |- match match match ?X with _ => _ end with _ => _ end with _ => _ end =>
+              consider X; intros
+          end.
+          { generalize (typ_cast_typ_eq _ _ _ _ _ H4). congruence. }
+          { repeat match goal with
+                 | _ : context [ match ?X with _ => _ end ] |- _ =>
+                   consider X; try congruence; intros
+                 | |- context [ match ?X with _ => _ end ] =>
+                   consider X; try congruence; intros
+               end; inv_all; subst; auto.
+            eapply H2.
+            clear - H1 H5.
+            assert (typeof_expr (typeof_funcs fs) (typeof_env us) x e = Some t).
+            eapply ExprD.typeof_expr_exprD'; eauto.
+            assert (typeof_expr (typeof_funcs fs) (typeof_env us) x e = Some x0).
+            eapply ExprD.typeof_expr_exprD'; eauto.
+            rewrite H in H0. inv_all; auto. } } }
+      { autorewrite with exprD_rw.
+        destruct (lookupAs us u t); auto. } }
+    { destruct t0; auto.
+      specialize (IHe1 t v); specialize (IHe2 t v).
+      repeat match goal with
+                 | _ : context [ match ?X with _ => _ end ] |- _ =>
+                   consider X; try congruence; intros
+                 | |- context [ match ?X with _ => _ end ] =>
+                   consider X; try congruence; intros
+               end; inv_all; subst; auto. }
+    { destruct t; auto.
+      specialize (IHe tvProp v).
+      repeat match goal with
+                 | _ : context [ match ?X with _ => _ end ] |- _ =>
+                   consider X; try congruence; intros
+                 | |- context [ match ?X with _ => _ end ] =>
+                   consider X; try congruence; intros
+               end; inv_all; subst; auto. }
+  Qed.
+End instantiate.
+
+Section mentionsU.
+  Section param.
+    Variable u : uvar.
+
+    Fixpoint mentionsU (e : expr) : bool :=
+      match e with
+        | Var _
+        | Func _ _ => false
+        | UVar u' => EqNat.beq_nat u u'
+        | App f e => if mentionsU f then true else mentionsU e
+        | Abs _ e => mentionsU e
+        | Equal _ e1 e2 => if mentionsU e1 then true else mentionsU e2
+        | Not e => mentionsU e
+      end.
+  End param.
+
+  Lemma mentionsU_lift : forall u e a b,
+    mentionsU u (lift a b e) = mentionsU u e.
+  Proof.
+    induction e; simpl; intros; rewrite lift_lift'; simpl; intuition;
+    repeat rewrite <- lift_lift' in *; intuition.
+    { destruct (NPeano.ltb v a); auto. }
+    { rewrite IHe1. rewrite IHe2. auto. }
+    { rewrite IHe1. rewrite IHe2. auto. }
+  Qed.
+
+  Theorem typeof_expr_mentionsU_strengthen : forall tfs tu e tg t',
+    mentionsU (length tu) e = false ->
+    typeof_expr tfs (tu ++ t' :: nil) tg e =
+    typeof_expr tfs tu tg e.
+  Proof.
+    induction e; simpl; intros;
+    repeat match goal with
+             | _ : context [ match ?X with _ => _ end ] |- _ =>
+               consider X; intros; try congruence
+             | H : _ |- _ =>
+               erewrite H by eauto
+           end; auto.
+    destruct (Compare_dec.lt_eq_lt_dec (length tu) u) as [ [ | ] | ].
+    { rewrite nth_error_past_end.
+      rewrite nth_error_past_end; auto.
+      omega. rewrite app_length. simpl. omega. }
+    { consider (EqNat.beq_nat (length tu) u); try congruence. }
+    { rewrite nth_error_app_L by auto. auto. }
+  Qed.
+
+  Lemma exprD'_mentionsU_strengthen : forall ts (fs : functions ts) tu u e,
+    mentionsU (length tu) e = false ->
+    forall tg t,
+    match ExprD.exprD' fs (tu ++ u :: nil) tg e t
+        , ExprD.exprD' fs tu tg e t
+    with
+      | None , None => True
+      | Some l , Some r => forall vs,
+                             l vs = r vs
+      | _ , _ => False
+    end.
+  Proof.
+    induction e; simpl; intros; autorewrite with exprD_rw;
+    repeat match goal with
+             | _ : context [ match ?X with _ => _ end ] |- _ =>
+               consider X; try congruence; intros
+           end.
+    { change (
+          let zzz z (pf : Some z = nth_error tg v) cast :=
+              (fun e : hlist (typD ts nil) tg =>
+                           match
+                             pf in (_ = t'')
+                             return
+                             (match t'' with
+                                | Some t0 => typD ts nil t0
+                                | None => unit
+                              end -> typD ts nil t)
+                           with
+                             | eq_refl => fun x : typD ts nil z => cast x
+                           end (hlist_nth e v))
+          in
+          match
+            match
+              nth_error tg v as z
+              return
+              (z = nth_error tg v ->
+               option (hlist (typD ts nil) tg -> typD ts nil t))
+            with
+              | Some z =>
+                fun pf : Some z = nth_error tg v =>
+                  match typ_cast_typ ts (fun x : Type => x) nil z t with
+                    | Some cast =>
+                      Some (zzz z pf cast)
+                    | None => None
+                  end
+              | None => fun _ : None = nth_error tg v => None
+            end eq_refl
+          with
+            | Some l =>
+              match
+                match
+                  nth_error tg v as z
+                  return
+                  (z = nth_error tg v ->
+                   option (hlist (typD ts nil) tg -> typD ts nil t))
+                with
+                  | Some z =>
+                    fun pf : Some z = nth_error tg v =>
+                      match typ_cast_typ ts (fun x : Type => x) nil z t with
+                        | Some cast =>
+                          Some (zzz z pf cast)
+                        | None => None
+                      end
+                  | None => fun _ : None = nth_error tg v => None
+                end eq_refl
+              with
+                | Some r => forall vs : hlist (typD ts nil) tg, l vs = r vs
+                | None => False
+              end
+            | None =>
+              match
+                match
+                  nth_error tg v as z
+                  return
+                  (z = nth_error tg v ->
+                   option (hlist (typD ts nil) tg -> typD ts nil t))
+                with
+                  | Some z =>
+                    fun pf : Some z = nth_error tg v =>
+                      match typ_cast_typ ts (fun x : Type => x) nil z t with
+                        | Some cast =>
+                          Some (zzz z pf cast)
+                        | None => None
+                      end
+                  | None => fun _ : None = nth_error tg v => None
+                end eq_refl
+              with
+                | Some _ => False
+                | None => True
+              end
+          end).
+      intro zzz; clearbody zzz; revert zzz.
+      gen_refl. destruct (nth_error tg v); auto.
+      destruct (typ_cast_typ ts (fun x : Type => x) nil t0 t); auto. }
+    { destruct (nth_error fs f); auto.
+      destruct (type_apply ts (fenv f0) l nil (ftype f0) (fdenote f0)); auto.
+      destruct (typ_cast_typ ts (fun x : Type => x) nil (instantiate_typ l (ftype f0)) t); auto. }
+    { rewrite typeof_env_app. simpl in *.
+      rewrite typeof_expr_mentionsU_strengthen by (rewrite typeof_env_length; auto).
+      consider (typeof_expr (typeof_funcs fs) (typeof_env tu) tg e1); auto; intros.
+      destruct t0; auto.
+      specialize (H0 eq_refl tg (tvArr t0_1 t0_2)).
+      specialize (IHe2 H1 tg t0_1).
+      repeat match goal with
+               | _ : context [ match ?X with _ => _ end ] |- _ =>
+                 consider X; try congruence; intros
+               | |- context [ match ?X with _ => _ end ] =>
+                 consider X; try congruence; intros
+             end; inv_all; subst; auto.
+      rewrite H4. rewrite IHe2. reflexivity. }
+    { destruct t0; auto.
+      specialize (IHe H (t :: tg) t0_2).
+      repeat match goal with
+               | _ : context [ match ?X with _ => _ end ] |- _ =>
+                 consider X; try congruence; intros
+               | |- context [ match ?X with _ => _ end ] =>
+                 consider X; try congruence; intros
+             end; inv_all; subst; auto.
+      eapply functional_extensionality; eauto. }
+    { unfold lookupAs.
+      destruct (Compare_dec.lt_eq_lt_dec (length tu) u0) as [ [ | ] | ].
+      { repeat rewrite nth_error_past_end by (try rewrite app_length; simpl; omega).
+        auto. }
+      { exfalso.
+        consider (EqNat.beq_nat (length tu) u0); congruence. } 
+      { rewrite nth_error_app_L by omega.
+        destruct (nth_error tu u0); auto.
+        destruct s.
+        destruct (TypesI.typ_cast (fun x0 : Type => x0) nil x t); auto. } }
+    { destruct t0; auto.
+      specialize (H0 eq_refl tg t); specialize (IHe2 H1 tg t).
+      repeat match goal with
+               | _ : context [ match ?X with _ => _ end ] |- _ =>
+                 consider X; try congruence; intros
+               | |- context [ match ?X with _ => _ end ] =>
+                 consider X; try congruence; intros
+             end; inv_all; subst; auto. }
+    { destruct t; auto.
+      specialize (IHe H tg tvProp).
+      repeat match goal with
+               | _ : context [ match ?X with _ => _ end ] |- _ =>
+                 consider X; try congruence; intros
+               | |- context [ match ?X with _ => _ end ] =>
+                 consider X; try congruence; intros
+              end; inv_all; subst; auto. }
+  Qed.
+
+End mentionsU.
